186    Chapter 7. THE ZETA FUNCTION AND PRIME NUMBER THEOREM

which holds for $0 \leq x < 1$, we find that

$$ \log \zeta(s) = \log \prod_{p} \frac{1}{1 - p^{-s}} = \sum_{p} \log \left( \frac{1}{1 - p^{-s}} \right) = \sum_{p,m} \frac{p^{-ms}}{m} . $$

Since the double sum converges absolutely, we need not specify the order of summation. See the Note at the end of this chapter. The formula then holds for all $\text{Re}(s) > 1$ by analytic continuation. Note that, by Theorem 6.2 in Chapter 3, $\log \zeta(s)$ is well defined in the simply connected half-plane $\text{Re}(s) > 1$, since $\zeta$ has no zeros there. Finally, it is clear that we have

$$ \sum_{p,m} \frac{p^{-ms}}{m} = \sum_{n=1}^{\infty} c_n n^{-s} , $$

where $c_n = 1/m$ if $n = p^m$ and $c_n = 0$ otherwise.

The proof of the theorem we shall give depends on a simple trick that is based on the following inequality.

**Lemma 1.4** *If $\theta \in \mathbb{R}$, then $3 + 4 \cos \theta + \cos 2\theta \geq 0$.*

This follows at once from the simple observation

$$ 3 + 4 \cos \theta + \cos 2\theta = 2(1 + \cos \theta)^2 . $$

**Corollary 1.5** *If $\sigma > 1$ and $t$ is real, then*

$$ \log |\zeta^3(\sigma) \zeta^4(\sigma + it) \zeta(\sigma + 2it)| \geq 0 . $$

*Proof.* Let $s = \sigma + it$ and note that

$$ \text{Re}(n^{-s}) = \text{Re}(e^{-(\sigma + it) \log n}) = e^{-\sigma \log n} \cos(t \log n) = n^{-\sigma} \cos(t \log n) . $$

Therefore,

$$ \begin{aligned} & \log |\zeta^3(\sigma) \zeta^4(\sigma + it) \zeta(\sigma + 2it)| \\ = & \ 3 \log |\zeta(\sigma)| + 4 \log |\zeta(\sigma + it)| + \log |\zeta(\sigma + 2it)| \\ = & \ 3 \text{Re}[\log \zeta(\sigma)] + 4 \text{Re}[\log \zeta(\sigma + it)] + \text{Re}[\log \zeta(\sigma + 2it)] \\ = & \ \sum c_n n^{-\sigma} (3 + 4 \cos \theta_n + \cos 2\theta_n) , \end{aligned} $$

where $\theta_n = t \log n$. The positivity now follows from Lemma 1.4, and the fact that $c_n \geq 0$.